src/arch/x64/vale.i.dfy
@@ -8,7 +8,7 @@ module x64_vale_i {
 import opened x64_def_s
 import opened words_and_bytes_i_temp = words_and_bytes_i
 
-type opr = operand // operand is a Vale keyword
+type opr = operand
 
 ////////////////////////////////////////////////////////////////////////
 //
@@ -18,8 +18,7 @@ type opr = operand // operand is a Vale keyword
 
 type va_int = int
 type va_bool = bool
-type va_operand_code = operand
-type va_operand_lemma = operand
+type va_operand = operand
 type va_code = code
 type va_codes = codes
 type va_state = State
@@ -56,8 +55,6 @@ function to_state(s:State):state { state(s.regs, s.xmms, s.flags, s.stack, s.hea
 //
 ////////////////////////////////////////////////////////////////////////
 
-function method va_op(o:va_operand_lemma):va_operand_code { o }
-
 function va_get_ok(s:va_state):bool { s.ok }
 //function va_get_reg32(r:x86reg, s:va_state):uint32 requires r in s.regs && IsUInt32(s.regs[r]) { s.regs[r] }
 function va_get_reg32(r:x86reg, s:va_state):uint32 requires r in s.regs { if IsUInt32(s.regs[r]) then s.regs[r] else lower64(s.regs[r]) }
@@ -83,43 +80,43 @@ function va_update_memory(sM:va_state, sK:va_state):va_state { sK.(heap := sM.he
 function va_update_flags(sM:va_state, sK:va_state):va_state { sK.(flags := sM.flags) }
 function va_update_stack(sM:va_state, sK:va_state):va_state { sK.(stack := sM.stack) }
 
-predicate va_is_src_imm8(o:opr) { o.OConst? && 0 <= o.n < 256 }
+predicate va_is_src_operand_imm8(o:opr) { o.OConst? && 0 <= o.n < 256 }
 
-predicate va_is_src_uint32(o:opr) { o.OConst? || (o.OReg? && !o.r.X86Xmm?) }
-predicate va_is_dst_uint32(o:opr) { o.OReg? && !o.r.X86Xmm? }
+predicate va_is_src_operand_uint32(o:opr) { o.OConst? || (o.OReg? && !o.r.X86Xmm?) }
+predicate va_is_dst_operand_uint32(o:opr) { o.OReg? && !o.r.X86Xmm? }
 
-predicate va_is_src_uint64(o:opr) { o.OConst? || (o.OReg? && !o.r.X86Xmm?) }
-predicate va_is_dst_uint64(o:opr) { o.OReg? && !o.r.X86Xmm? }
+predicate va_is_src_operand_uint64(o:opr) { o.OConst? || (o.OReg? && !o.r.X86Xmm?) }
+predicate va_is_dst_operand_uint64(o:opr) { o.OReg? && !o.r.X86Xmm? }
 
-predicate va_is_src_Quadword(o:opr) { o.OReg? && o.r.X86Xmm? && 0 <= o.r.xmm <= 7 }
-predicate va_is_dst_Quadword(o:opr) { o.OReg? && o.r.X86Xmm? && 0 <= o.r.xmm <= 7 }
+predicate va_is_src_operand_Quadword(o:opr) { o.OReg? && o.r.X86Xmm? && 0 <= o.r.xmm <= 7 }
+predicate va_is_dst_operand_Quadword(o:opr) { o.OReg? && o.r.X86Xmm? && 0 <= o.r.xmm <= 7 }
 
-function va_eval_op_imm8(s:va_state, o:opr):uint32
-    requires va_is_src_imm8(o);
+function va_eval_operand_imm8(s:va_state, o:opr):uint32
+    requires va_is_src_operand_imm8(o);
 {
     o.n
 }
 
-function va_eval_op_uint32(s:va_state, o:opr):uint32
-    requires va_is_src_uint32(o);
+function va_eval_operand_uint32(s:va_state, o:opr):uint32
+    requires va_is_src_operand_uint32(o);
 {
     eval_op32(to_state(s), o)
 }
 
-function va_eval_op_uint64(s:va_state, o:opr):uint64
-    requires va_is_src_uint64(o);
+function va_eval_operand_uint64(s:va_state, o:opr):uint64
+    requires va_is_src_operand_uint64(o);
 {
     eval_op64(to_state(s), o)
 }
 
-function va_eval_op_Quadword(s:va_state, o:opr):Quadword
-    requires va_is_src_Quadword(o);
+function va_eval_operand_Quadword(s:va_state, o:opr):Quadword
+    requires va_is_src_operand_Quadword(o);
     requires o.r.xmm in s.xmms;
 {
     Eval128BitOperand(to_state(s), o)
 }
 
-function va_update(o:opr, sM:va_state, sK:va_state):va_state
+function va_update_operand(o:opr, sM:va_state, sK:va_state):va_state
     requires o.OReg?;
     requires o.r in sM.regs;
     requires o.r.X86Xmm? ==> o.r.xmm in sM.xmms;
@@ -176,10 +173,12 @@ predicate va_ensure(b0:codes, b1:codes, s0:va_state, s1:va_state, sN:va_state)
  && x86_ValidState(s1)
 }
 
-function method va_op_const(n:uint32):opr { OConst(n) }
-function method va_op_reg32(r:x86reg):opr { OReg(r) }
-function method va_op_reg64(r:x86reg):opr { OReg(r) }
-function method va_op_Quadword(r:int):opr { OReg(X86Xmm(r)) }
+function method va_const_operand(n:uint32):opr { OConst(n) }
+function method va_op_operand_reg32(r:x86reg):opr { OReg(r) }
+function method va_op_operand_reg64(r:x86reg):opr { OReg(r) }
+function method va_op_operand_Quadword(r:int):opr { OReg(X86Xmm(r)) }
+function method va_op_cmp_reg32(r:x86reg):opr { OReg(r) }
+function method va_op_cmp_reg64(r:x86reg):opr { OReg(r) }
 
 function method va_cmp_eq(o1:opr, o2:opr):obool { OCmp(OEq, o1, o2) }
 function method va_cmp_ne(o1:opr, o2:opr):obool { OCmp(ONe, o1, o2) }
@@ -717,8 +716,8 @@ lemma va_lemma_block(b:codes, s0:va_state, r:va_state) returns(r1:va_state, c0:c
 lemma va_lemma_ifElse(ifb:obool, ct:code, cf:code, s:va_state, r:va_state) returns(cond:bool, s':va_state)
     requires !ifb.o1.OHeap? && !ifb.o2.OHeap?;
     requires x86_ValidState(s);
-    requires va_is_src_uint32(ifb.o1) && ValidSourceOperand(to_state(s), 32, ifb.o1);
-    requires va_is_src_uint32(ifb.o2) && ValidSourceOperand(to_state(s), 32, ifb.o2);
+    requires va_is_src_operand_uint32(ifb.o1) && ValidSourceOperand(to_state(s), 32, ifb.o1);
+    requires va_is_src_operand_uint32(ifb.o2) && ValidSourceOperand(to_state(s), 32, ifb.o2);
     requires eval_code(IfElse(ifb, ct, cf), s, r)
     ensures  if s.ok then
                     s'.ok
@@ -750,8 +749,8 @@ predicate va_whileInv(b:obool, c:code, n:int, r1:va_state, r2:va_state)
 }
 
 lemma va_lemma_while(b:obool, c:code, s:va_state, r:va_state) returns(n:nat, r':va_state)
-    requires va_is_src_uint32(b.o1);
-    requires va_is_src_uint32(b.o2);
+    requires va_is_src_operand_uint32(b.o1);
+    requires va_is_src_operand_uint32(b.o2);
     requires x86_ValidState(s);
     requires eval_code(While(b, c), s, r)
     ensures  evalWhileLax(b, c, n, to_state(s), to_state(r))
@@ -772,8 +771,8 @@ lemma va_lemma_while(b:obool, c:code, s:va_state, r:va_state) returns(n:nat, r':
 }
 
 lemma va_lemma_whileTrue(b:obool, c:code, n:nat, s:va_state, r:va_state) returns(s':va_state, r':va_state)
-    requires va_is_src_uint32(b.o1) && ValidSourceOperand(to_state(s), 32, b.o1);
-    requires va_is_src_uint32(b.o2) && ValidSourceOperand(to_state(s), 32, b.o2);
+    requires va_is_src_operand_uint32(b.o1) && ValidSourceOperand(to_state(s), 32, b.o1);
+    requires va_is_src_operand_uint32(b.o2) && ValidSourceOperand(to_state(s), 32, b.o2);
     requires n > 0
     requires evalWhileLax(b, c, n, to_state(s), to_state(r))
     ensures  x86_ValidState(s) ==> x86_ValidState(s');
@@ -782,7 +781,7 @@ lemma va_lemma_whileTrue(b:obool, c:code, n:nat, s:va_state, r:va_state) returns
     ensures  x86_ValidState(s) ==> if s.ok then x86_branchRelation(s, s', true) else s' == s;
     ensures  if s.ok && x86_ValidState(s) then
                     s'.ok
-                 && va_is_src_uint32(b.o1)
+                 && va_is_src_operand_uint32(b.o1)
                  && evalOBool(to_state(s), b)
                  && (s.heaplets == s'.heaplets == r'.heaplets)
              else
@@ -812,8 +811,8 @@ lemma va_lemma_whileTrue(b:obool, c:code, n:nat, s:va_state, r:va_state) returns
 }
 
 lemma va_lemma_whileFalse(b:obool, c:code, s:va_state, r:va_state) returns(r':va_state)
-    requires va_is_src_uint32(b.o1) && ValidSourceOperand(to_state(s), 32, b.o1);
-    requires va_is_src_uint32(b.o2) && ValidSourceOperand(to_state(s), 32, b.o2);
+    requires va_is_src_operand_uint32(b.o1) && ValidSourceOperand(to_state(s), 32, b.o1);
+    requires va_is_src_operand_uint32(b.o2) && ValidSourceOperand(to_state(s), 32, b.o2);
     requires evalWhileLax(b, c, 0, to_state(s), to_state(r))
     ensures  if s.ok then
                 (if x86_ValidState(s) then
